src/ocaml-output/FStar_TypeChecker_Env.ml
@@ -6199,7 +6199,6 @@ let (new_implicit_var_aux :
                       FStar_Syntax_Syntax.ctx_uvar_head = uu___2;
                       FStar_Syntax_Syntax.ctx_uvar_gamma = gamma;
                       FStar_Syntax_Syntax.ctx_uvar_binders = binders;
-                      FStar_Syntax_Syntax.ctx_uvar_typ = k;
                       FStar_Syntax_Syntax.ctx_uvar_reason = reason;
                       FStar_Syntax_Syntax.ctx_uvar_range = r;
                       FStar_Syntax_Syntax.ctx_uvar_meta = meta
