src/tactics/FStar.Tactics.Types.fst
@@ -35,7 +35,7 @@ module UF      = FStar.Syntax.Unionfind
 let goal_env g = g.goal_main_env
 let goal_witness g =
     FStar.Syntax.Syntax.mk (Tm_uvar (g.goal_ctx_uvar, ([], NoUseRange))) Range.dummyRange
-let goal_type g = g.goal_ctx_uvar.ctx_uvar_typ
+let goal_type g = U.ctx_uvar_typ g.goal_ctx_uvar
 
 let goal_with_env g env : goal =
     let c = g.goal_ctx_uvar in
@@ -49,6 +49,7 @@ let goal_of_ctx_uvar (g:goal) (ctx_u : ctx_uvar) : goal =
 let mk_goal env u o b l = {
     goal_main_env=env;
     goal_ctx_uvar=u;
+    goal_display_type=U.ctx_uvar_typ u;
     opts=o;
     is_guard=b;
     label=l;
@@ -82,11 +83,11 @@ let subst_goal subst goal =
     let ctx_uvar = {
         g with ctx_uvar_gamma=Env.rename_gamma subst g.ctx_uvar_gamma;
                ctx_uvar_binders=rename_binders subst g.ctx_uvar_binders;
-               ctx_uvar_typ=SS.subst subst g.ctx_uvar_typ;
     } in
-    { goal with goal_ctx_uvar = ctx_uvar }
+    { goal with goal_ctx_uvar = ctx_uvar;
+                goal_display_type = SS.subst subst goal.goal_display_type }
 
-let subst_proof_state subst ps =
+let subst_proof_display_state subst ps =
     if O.tactic_raw_binders ()
     then ps
     else { ps with goals = List.map (subst_goal subst) ps.goals
@@ -104,14 +105,14 @@ let tracepoint_with_psc psc ps : bool =
     if O.tactic_trace () || (ps.depth <= O.tactic_trace_d ()) then begin
         let ps = set_ps_psc psc ps in
         let subst = Cfg.psc_subst ps.psc in
-        ps.__dump (subst_proof_state subst ps) "TRACE"
+        ps.__dump (subst_proof_display_state subst ps) "TRACE"
     end;
     true
 
 let tracepoint ps : bool =
     if O.tactic_trace () || (ps.depth <= O.tactic_trace_d ()) then begin
         let subst = Cfg.psc_subst ps.psc in
-        ps.__dump (subst_proof_state subst ps) "TRACE"
+        ps.__dump (subst_proof_display_state subst ps) "TRACE"
     end;
     true
 
