src/typechecker/FStar.TypeChecker.Normalize.fst
@@ -3111,7 +3111,7 @@ let eta_expand (env:Env.env) (t:term) : term =
       let head, args = U.head_and_args t in
       begin match (SS.compress head).n with
       | Tm_uvar (u,s) ->
-        let formals, _tres = U.arrow_formals (SS.subst' s u.ctx_uvar_typ) in
+        let formals, _tres = U.arrow_formals (SS.subst' s (U.ctx_uvar_typ u)) in
         if List.length formals = List.length args
         then t
         else let _, ty, _ = env.typeof_tot_or_gtot_term ({env with lax=true; use_bv_sorts=true; expected_typ=None}) t true in
